Remove higher/big/ng references.

pulse/lib/core/PulseCore.Action.fst
@@ -448,7 +448,7 @@ let lift_eqs ()
   Sep.lift_emp_eq()
 
 let alloc
-    (#a:Type u#1)
+    (#a:Type)
     (#pcm:pcm a)
     (x:a{pcm.refine x})
 : act (ref a pcm) Atomic emp_inames emp (fun r -> pts_to r x)
@@ -468,7 +468,7 @@ let read
       emp_inames
       (pts_to r x)
       (fun v -> pts_to r (f v))
-= lift_pre_act1_act fun #ictx -> 
+= lift_pre_act3_act fun #ictx -> 
     ITA.lift_mem_action (Mem.select_refine #a #p r x f)
 
 let write
@@ -512,152 +512,6 @@ let gather
       (fun _ -> pts_to r (op pcm v0 v1))
 = lift_eqs(); lift_pre_act0_act fun #ictx ->
     ITA.lift_mem_action (Mem.gather_action #a #pcm r v0 v1)
-
-///////////////////////////////////////////////////////////////////
-// big refs
-///////////////////////////////////////////////////////////////////
-let big_pts_to #a #pcm r x = Sep.lift (Mem.big_pts_to #a #pcm r x)
-let timeless_big_pts_to #a #p r x = Sep.timeless_lift (Mem.big_pts_to #a #p r x)
-let big_pts_to_not_null #a #p r v = lift_pre_act0_act fun #ictx ->
-  ITA.lift_mem_action (Mem.big_pts_to_not_null_action #a #p r v)
-
-let big_alloc
-    (#a:Type)
-    (#pcm:pcm a)
-    (x:a{pcm.refine x})
-: act (ref a pcm) Atomic emp_inames emp (fun r -> big_pts_to r x)
-= lift_eqs(); lift_pre_act0_act fun #ictx ->
-    ITA.lift_mem_action (Mem.big_alloc_action #a #pcm x)
-
-let big_read
-    (#a:Type)
-    (#p:pcm a)
-    (r:ref a p)
-    (x:erased a)
-    (f:(v:a{compatible p x v}
-        -> GTot (y:a{compatible p y v /\
-                     FStar.PCM.frame_compatible p x v y})))
-: act (v:a{compatible p x v /\ p.refine v})
-      Atomic
-      emp_inames
-      (big_pts_to r x)
-      (fun v -> big_pts_to r (f v))
-= lift_pre_act2_act fun #ictx ->
-    lift_eqs();
-    ITA.lift_mem_action (Mem.big_select_refine#a #p r x f)
-
-let big_write
-    (#a:Type)
-    (#p:pcm a)
-    (r:ref a p)
-    (x y:Ghost.erased a)
-    (f:FStar.PCM.frame_preserving_upd p x y)
-: act unit
-      Atomic 
-      emp_inames
-      (big_pts_to r x)
-      (fun _ -> big_pts_to r y)
-= lift_pre_act0_act fun #ictx ->
-    ITA.lift_mem_action (Mem.big_upd_gen #a #p r x y f)
-
-let big_share
-    (#a:Type)
-    (#pcm:pcm a)
-    (r:ref a pcm)
-    (v0:FStar.Ghost.erased a)
-    (v1:FStar.Ghost.erased a{composable pcm v0 v1})
-: act unit
-      Ghost
-      emp_inames
-      (big_pts_to r (v0 `op pcm` v1))
-      (fun _ -> big_pts_to r v0 `star` big_pts_to r v1)
-= lift_eqs(); lift_pre_act0_act fun #ictx ->
-    ITA.lift_mem_action (Mem.big_split_action #a #pcm r v0 v1)
-
-let big_gather
-    (#a:Type)
-    (#pcm:pcm a)
-    (r:ref a pcm)
-    (v0:FStar.Ghost.erased a)
-    (v1:FStar.Ghost.erased a)
-: act (squash (composable pcm v0 v1))
-      Ghost
-      emp_inames
-      (big_pts_to r v0 `star` big_pts_to r v1)
-      (fun _ -> big_pts_to r (op pcm v0 v1))
-= lift_eqs(); lift_pre_act0_act fun #ictx ->
-    ITA.lift_mem_action (Mem.big_gather_action #a #pcm r v0 v1)
-
-let nb_pts_to #a #pcm r x = Sep.lift <| Mem.nb_pts_to #a #pcm r x
-let timeless_nb_pts_to #a #p r x = Sep.timeless_lift <| Mem.nb_pts_to #a #p r x
-let nb_pts_to_not_null #a #p r v = lift_pre_act0_act fun #ictx ->
-  ITA.lift_mem_action (Mem.nb_pts_to_not_null_action #a #p r v)
-
-let nb_alloc
-    (#a:Type)
-    (#pcm:pcm a)
-    (x:a{pcm.refine x})
-: act (ref a pcm) Atomic emp_inames emp (fun r -> nb_pts_to r x)
-= lift_eqs (); lift_pre_act0_act fun #ictx ->
-    ITA.lift_mem_action (Mem.nb_alloc_action #a #pcm x)
-
-let nb_read
-    (#a:Type)
-    (#p:pcm a)
-    (r:ref a p)
-    (x:erased a)
-    (f:(v:a{compatible p x v}
-        -> GTot (y:a{compatible p y v /\
-                     FStar.PCM.frame_compatible p x v y})))
-: act (v:a{compatible p x v /\ p.refine v})
-      Atomic
-      emp_inames
-      (nb_pts_to r x)
-      (fun v -> nb_pts_to r (f v))
-= lift_pre_act3_act fun #ictx ->
-    ITA.lift_mem_action (Mem.nb_select_refine #a #p r x f)
-
-let nb_write
-    (#a:Type)
-    (#p:pcm a)
-    (r:ref a p)
-    (x y:Ghost.erased a)
-    (f:FStar.PCM.frame_preserving_upd p x y)
-: act unit
-      Atomic 
-      emp_inames
-      (nb_pts_to r x)
-      (fun _ -> nb_pts_to r y)
-= lift_pre_act0_act fun #ictx ->
-    ITA.lift_mem_action <| Mem.nb_upd_gen #a #p r x y f
-
-let nb_share
-    (#a:Type)
-    (#pcm:pcm a)
-    (r:ref a pcm)
-    (v0:FStar.Ghost.erased a)
-    (v1:FStar.Ghost.erased a{composable pcm v0 v1})
-: act unit
-      Ghost
-      emp_inames
-      (nb_pts_to r (v0 `op pcm` v1))
-      (fun _ -> nb_pts_to r v0 `star` nb_pts_to r v1)
-= lift_eqs(); lift_pre_act0_act fun #ictx ->
-    ITA.lift_mem_action <| Mem.nb_split_action #a #pcm r v0 v1
-
-let nb_gather
-    (#a:Type)
-    (#pcm:pcm a)
-    (r:ref a pcm)
-    (v0:FStar.Ghost.erased a)
-    (v1:FStar.Ghost.erased a)
-: act (squash (composable pcm v0 v1))
-      Ghost
-      emp_inames
-      (nb_pts_to r v0 `star` nb_pts_to r v1)
-      (fun _ -> nb_pts_to r (op pcm v0 v1))
-= lift_eqs(); lift_pre_act0_act fun #ictx ->
-    ITA.lift_mem_action <| Mem.nb_gather_action #a #pcm r v0 v1
 
 
 ///////////////////////////////////////////////////////////////////
@@ -733,26 +587,10 @@ let ghost_pts_to_not_null #a #p r v =
   lift_pre_act0_act fun #ictx ->
   ITA.lift_mem_action (Mem.ghost_pts_to_not_null_action #a #p r v)
 let ghost_alloc #a #pcm x = let open Mem in lift_eqs (); lift_pre_act0_act fun #ictx -> ITA.lift_mem_action <| ghost_alloc #a #pcm x
-let ghost_read #a #p r x f = let open Mem in lift_eqs(); lift_pre_act1_act fun #ictx -> ITA.lift_mem_action <| ghost_read #a #p r x f
+let ghost_read #a #p r x f = let open Mem in lift_eqs(); lift_pre_act3_act fun #ictx -> ITA.lift_mem_action <| ghost_read #a #p r x f
 let ghost_write #a #p r x y f = let open Mem in lift_eqs(); lift_pre_act0_act fun #ictx -> ITA.lift_mem_action <| ghost_write #a #p r x y f
 let ghost_share #a #pcm r v0 v1 = let open Mem in lift_eqs(); lift_pre_act0_act fun #ictx -> ITA.lift_mem_action <| ghost_share #a #pcm r v0 v1
 let ghost_gather #a #pcm r v0 v1 = let open Mem in lift_eqs(); lift_pre_act0_act fun #ictx -> ITA.lift_mem_action <| ghost_gather #a #pcm r v0 v1
-
-let big_ghost_pts_to #a #p r x = Sep.lift (Mem.big_ghost_pts_to #a #p r x)
-let timeless_big_ghost_pts_to #a #p r x = Sep.timeless_lift (Mem.big_ghost_pts_to #a #p r x)
-let big_ghost_alloc #a #pcm x = let open Mem in lift_eqs(); lift_pre_act0_act fun #ictx -> ITA.lift_mem_action <| big_ghost_alloc #a #pcm x
-let big_ghost_read #a #p r x f = let open Mem in lift_eqs(); lift_pre_act2_act fun #ictx -> ITA.lift_mem_action <| big_ghost_read #a #p r x f
-let big_ghost_write #a #p r x y f = let open Mem in lift_eqs(); lift_pre_act0_act fun #ictx -> ITA.lift_mem_action <| big_ghost_write #a #p r x y f
-let big_ghost_share #a #pcm r v0 v1 = let open Mem in lift_eqs(); lift_pre_act0_act fun #ictx -> ITA.lift_mem_action <| big_ghost_share #a #pcm r v0 v1
-let big_ghost_gather #a #pcm r v0 v1 = let open Mem in lift_eqs(); lift_pre_act0_act fun #ictx -> ITA.lift_mem_action <| big_ghost_gather #a #pcm r v0 v1
-
-let nb_ghost_pts_to #a #p r x = Sep.lift (Mem.nb_ghost_pts_to #a #p r x)
-let timeless_nb_ghost_pts_to #a #p r x = Sep.timeless_lift (Mem.nb_ghost_pts_to #a #p r x)
-let nb_ghost_alloc #a #pcm x = let open Mem in lift_eqs(); lift_pre_act0_act fun #ictx -> ITA.lift_mem_action <| nb_ghost_alloc #a #pcm x
-let nb_ghost_read #a #p r x f = let open Mem in lift_eqs(); lift_pre_act3_act fun #ictx -> ITA.lift_mem_action <| nb_ghost_read #a #p r x f
-let nb_ghost_write #a #p r x y f = let open Mem in lift_eqs(); lift_pre_act0_act fun #ictx -> ITA.lift_mem_action <| nb_ghost_write #a #p r x y f
-let nb_ghost_share #a #pcm r v0 v1 = let open Mem in lift_eqs(); lift_pre_act0_act fun #ictx -> ITA.lift_mem_action <| nb_ghost_share #a #pcm r v0 v1
-let nb_ghost_gather #a #pcm r v0 v1 = let open Mem in lift_eqs(); lift_pre_act0_act fun #ictx -> ITA.lift_mem_action <| nb_ghost_gather #a #pcm r v0 v1
 
 
 let lift_erased #a ni_a #opens #pre #post f =
