pulse/lib/pulse/lib/Pulse.Lib.Reference.fst
@@ -17,58 +17,217 @@
 module Pulse.Lib.Reference
 #lang-pulse
 open Pulse.Lib.Core
-open Pulse.Main
-module H = Pulse.Lib.HigherReference
-friend Pulse.Lib.Array.Core
-inline_for_extraction
-let ref a = H.ref a
+module A = Pulse.Lib.Array.Basic
 
-inline_for_extraction
-let null (#a:Type u#0) : ref a = H.null
+let ref a = A.array a
 
-inline_for_extraction
+let null #a : ref a = A.null
+
 let is_null #a (r : ref a)
   : b:bool{b <==> r == null #a}
-= H.is_null r
+= A.is_null r
 
-let pts_to r = H.pts_to r
+let singleton #a (x:a) : Seq.seq a = Seq.create 1 x
+let singleton_inj #a (x: a) : Lemma (Seq.index (singleton x) 0 == x) [SMTPat (singleton x)] = ()
+let upd_singleton #a (x y: a) :
+    Lemma (Seq.upd (singleton x) 0 y == singleton y)
+      [SMTPat (Seq.upd (singleton x) 0 y)] =
+  assert Seq.equal (Seq.upd (singleton x) 0 y) (singleton y)
 
-let pts_to_timeless r p x = ()
+let pts_to (#a: Type u#a) (r:ref a) (#[T.exact (`1.0R)] p:perm) (n:a)
+= A.pts_to r #p (singleton n)
+let pts_to_timeless _ _ _ = ()
 
-let is_full_ref r = H.is_full_ref r
+let is_full_ref = A.is_full_array
 
-inline_for_extraction let alloc v = H.alloc v
-inline_for_extraction let read r = H.read r
-inline_for_extraction let op_Bang = read
-inline_for_extraction let write r = H.write r
-inline_for_extraction let op_Colon_Equals = write
-inline_for_extraction let free r = H.free r
+fn alloc u#a (#a: Type u#a) {| small_type u#a |} (x:a)
+  returns r:ref a
+  ensures pts_to r x
+  ensures pure (is_full_ref r)
+{
+  let r = A.alloc x 1sz;
+  fold (pts_to r #1.0R x);
+  r
+}
 
-let share r = H.share r
-let gather r = H.gather r
+fn read u#a (#a: Type u#a) (r:ref a) (#n:erased a) (#p:perm)
+  preserves r |-> Frac p n
+  returns  x : a
+  ensures  rewrites_to x n
+{
+  unfold pts_to r #p n;
+  let x = A.(r.(0sz));
+  fold (pts_to r #p n);
+  x
+}
+
+inline_for_extraction
+let ( ! ) #a = read #a
+
+fn write u#a (#a: Type u#a) (r:ref a) (x:a) (#n:erased a)
+  requires r |-> n
+  ensures  r |-> x
+{
+  unfold pts_to r #1.0R n;
+  A.(r.(0sz) <- x);
+  fold pts_to r #1.0R x;
+}
+
+inline_for_extraction
+let ( := ) #a = write #a
 
 
-let with_local init = H.with_local init
+fn free u#a (#a: Type u#a) (r:ref a) (#n:erased a)
+  requires pts_to r #1.0R n
+  requires pure (is_full_ref r)
+{
+  unfold pts_to r #1.0R n;
+  A.free r;
+}
+
+ghost
+fn share u#a (#a: Type u#a) (r:ref a) (#v:erased a) (#p:perm)
+  requires pts_to r #p v
+  ensures pts_to r #(p /. 2.0R) v ** pts_to r #(p /. 2.0R) v
+{
+  unfold pts_to r #p v;
+  A.share r;
+  fold (pts_to r #(p /. 2.0R) v);
+  fold (pts_to r #(p /. 2.0R) v);
+}
+
+ghost
+fn gather u#a (#a: Type u#a) (r:ref a) (#x0 #x1:erased a) (#p0 #p1:perm)
+  requires pts_to r #p0 x0 ** pts_to r #p1 x1
+  ensures pts_to r #(p0 +. p1) x0 ** pure (x0 == x1)
+{ 
+  unfold pts_to r #p0 x0;
+  unfold pts_to r #p1 x1;
+  A.gather r;
+  fold (pts_to r #(p0 +. p1) x0)
+}
+
+fn with_local u#a u#b
+  (#a:Type u#a) {| small_type u#a |}
+  (init:a)
+  (#pre:slprop)
+  (#ret_t:Type u#b)
+  (#post:ret_t -> slprop)
+  (body:(r:ref a) -> stt ret_t (pre ** pts_to r init)
+                               (fun v -> post v ** (exists* (x:a). pts_to r x)))
+  : stt ret_t pre (fun r -> post r) =
+{
+  let x = alloc init;
+  let r = body x;
+  free x;
+  r
+}
+
+ghost
+fn pts_to_injective_eq
+    u#a (#a: Type u#a)
+    (#p0 #p1:perm)
+    (#v0 #v1:a)
+    (r:ref a)
+  requires pts_to r #p0 v0 ** pts_to r #p1 v1
+  ensures (pts_to r #p0 v0 ** pts_to r #p1 v1) ** pure (v0 == v1)
+{
+  unfold pts_to r #p0 v0;
+  unfold pts_to r #p1 v1;
+  A.pts_to_injective_eq r;
+  fold pts_to r #p0 v0;
+  fold pts_to r #p1 v1;
+}
 
 
-let pts_to_injective_eq r = H.pts_to_injective_eq r
-let pts_to_perm_bound r = H.pts_to_perm_bound r
-let pts_to_not_null r = H.pts_to_not_null r
+ghost
+fn pts_to_perm_bound u#a (#a: Type u#a) (#p:_) (r:ref a) (#v:a)
+  requires pts_to r #p v
+  ensures pts_to r #p v ** pure (p <=. 1.0R)
+{
+  unfold pts_to r #p v;
+  A.pts_to_perm_bound r;
+  fold pts_to r #p v;
+}
 
-fn replace (#a:Type0) (r:ref a) (x:a) (#v:erased a)
-  requires pts_to r v
-  returns y:a
-  ensures pts_to r x ** pure (y == reveal v)
+ghost
+fn pts_to_not_null u#a (#a: Type u#a) (#p:_) (r:ref a) (#v:a)
+  preserves r |-> Frac p v
+  ensures  pure (not (is_null #a r))
+{
+  unfold pts_to r #p v;
+  A.pts_to_not_null r;
+  fold pts_to r #p v;
+}
+
+let to_array_ghost r = r
+
+unobservable
+fn to_array u#a (#a: Type u#a) (r: ref a) #p (#v: erased a)
+  requires r |-> Frac p v
+  returns arr: array a
+  ensures rewrites_to arr (to_array_ghost r)
+  ensures arr |-> Frac p (seq![reveal v])
+  ensures pure (length arr == 1)
+{
+  unfold pts_to r #p v;
+  pts_to_len r;
+  assert pure (Seq.equal seq![reveal v] (singleton (reveal v)));
+  r
+}
+
+ghost
+fn return_to_array u#a (#a: Type u#a) (r: ref a) #p (#v: Seq.seq a)
+  requires to_array_ghost r |-> Frac p v
+  requires pure (length (to_array_ghost r) == 1)
+  returns _: squash (Seq.length v == 1)
+  ensures r |-> Frac p (Seq.index v 0)
+{
+  pts_to_len r;
+  assert pure (singleton (Seq.Base.index v 0) `Seq.equal` v);
+  fold pts_to r #p (Seq.index v 0);
+}
+
+let array_at_ghost arr i = gsub arr i (i+1)
+
+unobservable
+fn array_at u#a (#a: Type u#a) (arr: array a) (i: SizeT.t) #p (#v: erased (Seq.seq a) { SizeT.v i < length arr /\ length arr == Seq.length v }) #mask
+  requires pts_to_mask arr #p v mask
+  requires pure (mask (SizeT.v i))
+  returns r: ref a
+  ensures rewrites_to r (array_at_ghost arr (SizeT.v i))
+  ensures r |-> Frac p (Seq.index v (SizeT.v i))
+  ensures pts_to_mask arr #p v (fun k -> mask k /\ k <> SizeT.v i)
+{
+  let res = sub arr i (SizeT.v i + 1);
+  mask_ext res (singleton (Seq.index v (SizeT.v i))) (fun _ -> True);
+  from_mask res;
+  fold pts_to res #p (Seq.index v (SizeT.v i));
+  mask_mext arr (fun k -> mask k /\ k <> SizeT.v i);
+  res
+}
+
+ghost
+fn return_array_at u#a (#a: Type u#a) (arr: array a) (i: nat) (#p: perm) (#v: a) (#v': Seq.seq a { i < length arr /\ length arr == Seq.length v' }) (#mask: nat->prop)
+  requires array_at_ghost arr i |-> Frac p v
+  requires pts_to_mask arr #p v' mask
+  requires pure (~(mask i))
+  ensures pts_to_mask arr #p (Seq.upd v' i v) (fun k -> mask k \/ k == i)
+{
+  unfold pts_to (array_at_ghost arr i) #p v;
+  to_mask (array_at_ghost arr i);
+  gsub_elim arr i (i+1);
+  join_mask arr;
+  mask_ext arr (Seq.upd v' i v) (fun k -> mask k \/ k == i);
+}
+
+fn replace u#a (#a:Type u#a) (r:ref a) (x:a) (#v:erased a)
+  requires r |-> v
+  returns  res: a
+  ensures  r |-> x
+  ensures  rewrites_to res v
 {
   let y = !r;
   r := x;
   y
 }
-
-let to_array_ghost r = H.to_array_ghost r
-inline_for_extraction let to_array r = H.to_array r
-let return_to_array r = H.return_to_array r
-
-let array_at_ghost arr i = H.array_at_ghost arr i
-inline_for_extraction let array_at arr = H.array_at arr
-let return_array_at arr = H.return_array_at arr
