pulse/src/checker/Pulse.Extract.Main.fst
@@ -414,6 +414,8 @@ let unit_binder (ppname: string) =
     qual = R.Q_Explicit;
   }
 
+let small_type0 = tm_constant R.C_Unit
+
 open Pulse.Syntax.Naming
 let rec extract_dv g (p:st_term) : T.Tac R.term =
   if is_erasable p then ECL.mk_return ECL.unit_tm
@@ -482,8 +484,8 @@ let rec extract_dv g (p:st_term) : T.Tac R.term =
 
     | Tm_WithLocal { binder; initializer; body } ->
       let b' = extract_dv_binder binder None in
-      let allocator = R.mk_app (R.pack_ln (R.Tv_FVar (R.pack_fv ["Pulse"; "Lib"; "Reference"; "alloc"])))
-        [get_type_of_ref binder.binder_ty, R.Q_Implicit; initializer, R.Q_Explicit] in
+      let allocator = R.mk_app (R.pack_ln (R.Tv_UInst (R.pack_fv ["Pulse"; "Lib"; "Reference"; "alloc"]) [u0]))
+        [get_type_of_ref binder.binder_ty, R.Q_Implicit; small_type0, R.Q_Explicit; initializer, R.Q_Explicit] in
       let g, x = extend_env'_binder g binder in
       let body = extract_dv g (open_st_term_nv body x) in
       ECL.mk_let b' allocator (close_term body x._2)
@@ -495,8 +497,8 @@ let rec extract_dv g (p:st_term) : T.Tac R.term =
       //
       // This is parsed by Pulse2Rust
       //
-      let allocator = R.mk_app (R.pack_ln (R.Tv_FVar (R.pack_fv ["Pulse"; "Lib"; "Array"; "Core"; "alloc"])))
-        [get_type_of_array binder.binder_ty, R.Q_Implicit; initializer, R.Q_Explicit; length, R.Q_Explicit] in
+      let allocator = R.mk_app (R.pack_ln (R.Tv_UInst (R.pack_fv ["Pulse"; "Lib"; "Array"; "PtsTo"; "alloc"]) [u0]))
+        [get_type_of_array binder.binder_ty, R.Q_Implicit; small_type0, R.Q_Explicit; initializer, R.Q_Explicit; length, R.Q_Explicit] in
       let g, x = extend_env'_binder g binder in
       let body = extract_dv g (open_st_term_nv body x) in
       ECL.mk_let b' allocator (close_term body x._2)
